WIP integration experiment

examples/http/Main.hs
@@ -6,19 +6,29 @@ import Network.Socket
 
 main :: IO ()
 main = do
-    sock <- socket AF_INET Stream 0    -- create socket
-    setSocketOption sock ReuseAddr 1   -- make socket immediately reusable - eases debugging.
-    bind sock (SockAddrInet 4242 iNADDR_ANY)   -- listen on TCP port 4242.
-    listen sock 2                              -- set a max of 2 queued connections
-    mainLoop sock                              -- unimplemented
+  sock <- socket AF_INET Stream 0    -- create new Socket on server
+  setSocketOption sock ReuseAddr 1   -- make socket immediately reusable - eases debugging.
+  bind sock (SockAddrInet 4242 iNADDR_ANY)   -- listen on TCP port 4242.
+  listen sock 2                              -- set a max of 2 queued connections
+  mainLoop sock                              -- unimplemented
 
 mainLoop :: Socket -> IO ()
 mainLoop sock = do
-    conn <- accept sock     -- accept a connection and handle it
-    runConn conn            -- run our server's logic
-    mainLoop sock           -- repeat
+  -- `accept` returns a (conn, addr)
+  -- where `conn` is the new socket object, usable to send and receive the data.
+  -- `addr` is the address of the socket on the other end of the connection.
+  --
+  -- In order to accept the connection and handle it, the socket must be
+  -- 1. Bound to an address
+  -- 2. Listening for a connection
+  conn <- accept sock     -- accept a connection and handle it
+  runConn conn            -- run our server's logic
+  mainLoop sock           -- repeat
 
 runConn :: (Socket, SockAddr) -> IO ()
 runConn (sock, _) = do
-    send sock "Hello World!\n"
-    close sock
+  -- Send data to socket. Socket must be connected to a remote socket. returns
+  -- number of bytes sent. Apps are responsible for ensuring all data has been sent.
+  send sock "Hello World!\n"
+  -- `close` does not throw exceptions
+  close sock
