examples/http/manual/NetworkTypes.v
@@ -1,16 +1,375 @@
 Require GHC.Base.
 Require GHC.Num.
 
-Axiom Socket : Type.
-Axiom SockAddr : Type.
-Axiom SocketOption : Type.
-Axiom HostAddress : Type.
-Axiom ProtocolNumber : Type.
-Axiom SocketType : Type.
-Axiom Family : Type.
-Axiom AF_INET : Family.
-Axiom Stream : SocketType.
-Axiom SockAddrInet : Num.Int -> HostAddress -> SockAddr.
-Axiom ReuseAddr : SocketOption.
-Axiom iNADDR_ANY : HostAddress.
+From Coq Require Import
+     ZArith
+     String
+     List
+     FunctionalExtensionality
+     ProofIrrelevance.
+(* Axiomatized network types. *)
+Section NetworkTypes.
 
+  Axiom Socket : Type.
+  Axiom SockAddr : Type.
+  Axiom SocketOption : Type.
+  Axiom HostAddress : Type.
+  Axiom ProtocolNumber : Type.
+  Axiom SocketType : Type.
+  Axiom Family : Type.
+  Axiom AF_INET : Family.
+  Axiom Stream : SocketType.
+  Axiom SockAddrInet : Num.Int -> HostAddress -> SockAddr.
+  Axiom ReuseAddr : SocketOption.
+  Axiom iNADDR_ANY : HostAddress.
+
+End NetworkTypes.
+
+Module SocketModel.
+
+  (* POSIX socket API constants *)
+  Definition MAX_FD : Z := 4096.
+
+  Definition AF_INET : Z := 2.
+
+  Definition SOCK_STREAM : Z := 1.
+  Definition SOCK_DGRAM : Z := 2.
+  Definition SOCK_RAW : Z := 3.
+  Definition SOCK_RD : Z := 4.
+  Definition SOCK_SEQPACKET : Z := 5.
+  Definition SOCK_PACKET : Z := 10.
+
+  Definition INVALID_SOCKET : Z := -1.
+  Definition FD_SETSIZE : Z := 1024.
+
+  Open Scope Z.
+
+  Parameter is_fd: Z -> Prop.
+  Axiom fd_bound: forall i, is_fd i -> 0 <= i <= MAX_FD.
+  Axiom zero_is_fd : is_fd 0.
+
+  Variant connection_id : Type := Connection (c : nat).
+
+  Definition eqb_connection_id :
+    forall c1 c2 : connection_id, {c1 = c2} + {c1 <> c2}.
+  Proof.
+    intros [] [].
+    destruct (c =? c0)%nat eqn:H; auto.
+    - apply beq_nat_true in H.
+      subst; auto.
+    - apply beq_nat_false in H.
+      right.
+      unfold not; intros conn_eq; inversion conn_eq; contradiction.
+  Defined.
+
+  Record endpoint_id : Type := Endpoint
+    { port_number : Z;
+    }.
+
+  Record sockfd: Type :=
+    { descriptor : Z;
+      is_descriptor: is_fd descriptor }.
+
+  Definition fd_eqb (fd1 fd2 : sockfd) : bool :=
+    descriptor fd1 =? descriptor fd2.
+
+  Lemma is_fd_irrelevant: forall fd1 fd2,
+      descriptor fd1 = descriptor fd2 -> fd1 = fd2.
+  Proof.
+    intros [] [] Heqb.
+    simpl in Heqb.
+    pose proof proof_irrelevance.
+    subst.
+    specialize (H (is_fd descriptor1) is_descriptor0 is_descriptor1).
+    subst.
+    reflexivity.
+  Qed.
+
+  Variant socket_status :=
+  | ClosedSocket
+  | OpenedSocket
+  | BoundSocket (addr : endpoint_id)
+  | ListeningSocket (addr : endpoint_id)
+  | ConnectedSocket (conn : connection_id).
+
+  Record SocketMap : Type :=
+    { lookup_socket :> sockfd -> socket_status }.
+
+  Lemma lookup_descriptor:
+    forall (api_st : SocketMap) (fd1 fd2 : sockfd),
+      descriptor fd1 = descriptor fd2 ->
+      lookup_socket api_st fd1 = lookup_socket api_st fd2.
+  Proof.
+    intros ? ? ? H.
+    apply is_fd_irrelevant in H.
+    subst.
+    reflexivity.
+  Qed.
+
+  Definition connection_of_fd (api_st: SocketMap) (fd : sockfd)
+    : option connection_id :=
+    match lookup_socket api_st fd with
+    | ConnectedSocket conn => Some conn
+    | _ => None
+    end.
+
+  Definition endpoint_of_fd (api_st: SocketMap) (fd : sockfd)
+    : option endpoint_id :=
+    match lookup_socket api_st fd with
+    | BoundSocket addr => Some addr
+    | ListeningSocket addr => Some addr
+    | _ => None
+    end.
+
+  Definition update_socket_state
+             (api_st: SocketMap)
+             (fd : sockfd) (new_status: socket_status) :
+    SocketMap :=
+    {| lookup_socket fd' :=
+         if Z.eqb (descriptor fd) (descriptor fd') then new_status
+         else lookup_socket api_st fd';
+    |}.
+
+  Lemma lookup_update_socket_neq
+        (api_st : SocketMap)
+        (fd : sockfd) (new_status : socket_status)
+        (fd' : sockfd):
+    descriptor fd <> descriptor fd' ->
+    lookup_socket (update_socket_state api_st fd new_status) fd' =
+    lookup_socket api_st fd'.
+  Proof.
+    intros.
+    unfold update_socket_state.
+    simpl.
+    destruct (descriptor fd =? descriptor fd') eqn:Heq.
+    rewrite Z.eqb_eq in Heq;
+      exfalso; apply H; auto.
+    reflexivity.
+  Qed.
+
+  Lemma lookup_update_socket_eq
+        (api_st : SocketMap)
+        (fd : sockfd) (new_status : socket_status)
+        (fd' : sockfd):
+    descriptor fd = descriptor fd' ->
+    lookup_socket (update_socket_state api_st fd new_status) fd' = new_status.
+  Proof.
+    intros.
+    unfold update_socket_state.
+    simpl.
+    rewrite <- Z.eqb_eq in H.
+    rewrite H.
+    reflexivity.
+  Qed.
+
+  Lemma lookup_update_socket_notIn
+        (api_st : SocketMap)
+        (fd : sockfd) (new_status : socket_status)
+        (fds : list sockfd):
+    ~In fd fds ->
+    (forall fd', In fd' fds ->
+            lookup_socket (update_socket_state api_st fd new_status) fd'
+            = api_st fd').
+  Proof.
+    intros H.
+    intros fd' fd'_in.
+    rewrite lookup_update_socket_neq; trivial.
+    unfold not; intro Hcontra.
+    apply is_fd_irrelevant in Hcontra.
+    subst fd.
+    contradiction.
+  Qed.
+
+  Lemma lookup_update_socket_In
+        (api_st : SocketMap)
+        (fd : sockfd) (new_status : socket_status)
+        (fds : list sockfd):
+    In fd fds ->
+    (forall fd', ~In fd' fds ->
+            lookup_socket (update_socket_state api_st fd new_status) fd'
+            = api_st fd').
+  Proof.
+    intros H.
+    intros fd' fd'_in.
+    rewrite lookup_update_socket_neq; trivial.
+    unfold not; intro Hcontra.
+    apply is_fd_irrelevant in Hcontra.
+    subst fd.
+    contradiction.
+  Qed.
+
+  Lemma socket_extensionality (api_st1 api_st2 : SocketMap):
+    (forall fd, lookup_socket api_st1 fd = lookup_socket api_st2 fd) ->
+    api_st1 = api_st2.
+  Proof.
+    intros Hlookup.
+    destruct api_st1, api_st2.
+    f_equal.
+    apply functional_extensionality.
+    intros fd'.
+    apply Hlookup; auto.
+  Qed.
+
+  Lemma restore_update_socket
+        (api_st0 : SocketMap)
+        (fd : sockfd) (st st' : socket_status):
+    lookup_socket api_st0 fd = st ->
+    let api_st1 := update_socket_state api_st0 fd st' in
+    let api_st2 := update_socket_state api_st1 fd st in
+    api_st0 = api_st2.
+  Proof.
+    intros Hst.
+    apply socket_extensionality.
+    intros fd'.
+    destruct (descriptor fd =? descriptor fd') eqn:Hfd.
+    {
+      apply Z.eqb_eq in Hfd.
+      pose proof Hfd as Hfd'.
+      apply lookup_descriptor with (api_st := api_st0) in Hfd.
+      rewrite lookup_update_socket_eq by assumption.
+      subst.
+      rewrite Hfd.
+      reflexivity.
+    }
+
+    apply Z.eqb_neq in Hfd.
+    rewrite lookup_update_socket_neq by assumption.
+    rewrite lookup_update_socket_neq by assumption.
+    trivial.
+  Qed.
+
+  Lemma update_socket_id
+        (api_st : SocketMap) (fd : sockfd):
+    api_st = update_socket_state api_st fd (lookup_socket api_st fd).
+  Proof.
+    intros.
+    unfold update_socket_state, lookup_socket.
+    destruct api_st eqn:Hst.
+    f_equal.
+    apply functional_extensionality.
+    intros fd'.
+    destruct (descriptor fd =? descriptor fd') eqn:Heq; auto.
+    rewrite Z.eqb_eq in Heq.
+    apply lookup_descriptor with (api_st := api_st) in Heq.
+    subst.
+    auto.
+  Qed.
+
+  Definition consistent_world (api_st : SocketMap) :=
+    forall fd1 fd2 id1 id2,
+      lookup_socket api_st fd1 = ConnectedSocket id1 ->
+      lookup_socket api_st fd2 = ConnectedSocket id2 ->
+      fd1 <> fd2 -> id1 <> id2.
+
+  Lemma consistent_world_monotone
+        (api_st: SocketMap) (st: socket_status):
+    consistent_world api_st ->
+    ~(exists id, st = ConnectedSocket id) ->
+    forall fd, consistent_world (update_socket_state api_st fd st).
+  Proof.
+    intros Hconsistent Hstatus fd
+           fd1 fd2 id1 id2
+           Hlookup1 Hlookup2 fd_neq.
+
+    destruct (descriptor fd =? descriptor fd1) eqn:Hfd1.
+    {
+      pose proof Hfd1 as fds_eq.
+      rewrite Z.eqb_eq in fds_eq.
+      apply is_fd_irrelevant in fds_eq.
+      simpl in Hlookup1.
+      rewrite Hfd1 in *.
+      subst.
+      exfalso.
+      apply Hstatus.
+      exists id1.
+      reflexivity.
+    }
+
+    destruct (descriptor fd =? descriptor fd2) eqn:Hfd2.
+    {
+      pose proof Hfd2 as fds_eq.
+      rewrite Z.eqb_eq in fds_eq.
+      apply is_fd_irrelevant in fds_eq.
+      simpl in Hlookup2.
+      rewrite Hfd2 in *.
+      subst.
+      exfalso.
+      apply Hstatus.
+      exists id2.
+      reflexivity.
+    }
+
+    rewrite Z.eqb_neq in *.
+
+    rewrite lookup_update_socket_neq in *; auto.
+    eauto.
+  Qed.
+
+End SocketModel.
+
+Module FDSet.
+
+  Import SocketModel.
+
+  Definition FD_Set : Type := list sockfd.
+
+  Definition insert_fd (fd : sockfd) (set : FD_Set) : FD_Set :=
+    if List.existsb (fd_eqb fd) set
+    then set
+    else (fd :: set).
+
+  Definition remove_fd (fd : sockfd) (set : FD_Set) : FD_Set :=
+    List.filter (fun fd' => negb (fd_eqb fd fd')) set.
+
+  Definition fd_subset (fdset1 fdset2 : FD_Set) : Prop :=
+    List.incl (List.map descriptor fdset1)
+              (List.map descriptor fdset2).
+
+  Lemma fd_subset_refl:
+    forall (fd_set : FD_Set), fd_subset fd_set fd_set.
+  Proof.
+    intros; unfold fd_subset; apply incl_refl.
+  Qed.
+
+  Lemma fd_subset_trans:
+    forall (fd_set1 fd_set2 fd_set3: FD_Set),
+      fd_subset fd_set1 fd_set2 ->
+      fd_subset fd_set2 fd_set3 ->
+      fd_subset fd_set1 fd_set3.
+  Proof.
+    unfold fd_subset; intros; eapply incl_tran; eassumption.
+  Qed.
+
+  Lemma fd_subset_insert1:
+    forall (fd_set1 fd_set2 : FD_Set) (fd : sockfd),
+      fd_subset fd_set1 fd_set2 ->
+      In (descriptor fd) (map descriptor fd_set2) ->
+      fd_subset (insert_fd fd fd_set1) fd_set2.
+  Proof.
+    intros.
+    unfold insert_fd.
+    destruct (existsb (fd_eqb fd)); trivial.
+    unfold fd_subset.
+    simpl.
+    apply incl_cons; trivial.
+  Qed.
+
+  Lemma fd_subset_insert2:
+    forall (fd_set1 fd_set2 : FD_Set) (fd : sockfd),
+      fd_subset fd_set1 fd_set2 ->
+      fd_subset fd_set1 (insert_fd fd fd_set2).
+  Proof.
+    intros; unfold insert_fd; destruct (existsb (fd_eqb fd)); trivial.
+    unfold fd_subset in *.
+    simpl.
+    apply incl_tl; assumption.
+  Qed.
+
+End FDSet.
+
+Module SockAddr.
+
+  Record SockAddr :=
+    { sin_family : Z ; sin_port : Z ; sin_addr : Z }.
+
+End SockAddr.
