examples/http/manual/IO-old.v
@@ -1,0 +1,474 @@
+
+From ExtLib.Structures Require Functor Applicative Monad.
+From ITree Require Import
+     ITree
+     Basics.Basics
+     Events.State.
+
+From Coq Require Import Lists.List
+     String.
+
+Require Import NetworkTypes.
+Require Import DeepWeb.Lib.Socket DeepWeb.Lib.SocketInterface DeepWeb.Lib.Util Map DeepWeb.Lib.NetworkInterface.
+
+Import SocketAPI. 
+Import ListNotations.
+
+(** *Modeling network relevant I/O operations.
+
+  (An experiment.)
+  ""Relevant"" events and effects were crafted from the Network.Socket
+  library documentation.
+
+   https://hackage.haskell.org/package/network-3.1.1.1/docs/Network-Socket.html
+
+ *)
+
+Definition Socket := sockfd.
+
+(* ====================================================== *)
+(** *Haskell Network Events
+
+   Network.v defines the corresponding embeddings of
+   these uninterpreted events into ITrees.
+
+   These are "axiomiatized" translations of relevant network effects, which
+   can be automatically generated.
+ *)
+Inductive haskE : Type -> Type :=
+| SendE : Socket -> bytes -> haskE Num.Int
+| CloseE : Socket -> haskE unit
+| AcceptE : Socket -> haskE (Socket * SockAddr)
+| ListenE : Socket -> Num.Int -> haskE unit
+| BindE : Socket -> SockAddr -> haskE unit
+| SocketE : Family -> SocketType -> Num.Int -> haskE Socket
+| SetSocketOptionE : Socket -> SocketOption -> Num.Int -> haskE unit.
+
+(* ====================================================== *)
+(** *Composing IO Events
+
+   Alternatively, if we wanted to model _different IO events_, we can
+   use the sum operator to combine different events.
+
+   For instance, we can define the following:
+
+   (* Read/write event to STDIN. *)
+   Inductive rwE : Type -> Type :=
+   | ReadEff : rwE unit
+   | WriteEff : rwE unit
+   .
+
+   Definition ioE := rwE +' networkE.
+
+   Using subevents, we can also compose different events. For now, we
+   only focus on single-threaded network events.
+ *)
+Require Import ITree.Events.Nondeterminism ITree.Events.Exception.
+
+Section OpenUnion.
+  Generalizable Variables A B C D E.
+  Class Convertible (A B : Type -> Type) :=
+    { convert : forall {X}, A X -> B X }.
+
+  (* Don't try to guess. *)
+  Instance fluid_id A : Convertible A A | 0 :=
+    { convert X a := a }.
+
+  (* Destructure sums. *)
+  Instance fluid_sum `{Convertible A C} `{Convertible B C}
+    : Convertible (sum1 A B) C | 7 :=
+    { convert X ab :=
+        match ab with
+        | inl1 a => convert a
+        | inr1 b => convert b
+        end }.
+
+  (* Lean left by default for no reason. *)
+  Instance fluid_left `{Convertible A B} C
+    : Convertible A (sum1 B C) | 8 :=
+    { convert X a := inl1 (convert a) }.
+
+  (* Very incoherent instances. *)
+  Instance fluid_right `{Convertible A C} B
+    : Convertible A (sum1 B C) | 9 :=
+    { convert X a := inr1 (convert a) }.
+
+  Instance fluid_empty A : Convertible void1 A :=
+    { convert X v := match v with end }.
+
+  Definition lift {E F X} `{Convertible E F} : itree E X -> itree F X :=
+    @translate _ _ (@convert _ _ _) _.
+
+  Class Embed X Y :=
+    { embed : X -> Y }.
+
+  Instance Embed_fun A X Y `{Embed X Y} : Embed (A -> X) (A -> Y) :=
+    { embed := fun x a => embed (x a) }.
+
+  Instance Embed_eff E F X `{Convertible E F} : Embed (E X) (itree F X) :=
+    { embed := fun e => trigger (convert e) }.
+
+  Arguments embed {X Y _} e.
+
+End OpenUnion.
+
+  Notation "E -< F" := (Convertible E F)
+  (at level 92, left associativity) : type_scope.
+
+  Definition or {E X} `{nondetE -< E} (k1 k2 : itree E X) : itree E X :=
+    Vis (convert Or) (fun x : bool => if x then k1 else k2).
+
+Definition ioE := haskE +' (exceptE string) +' nondetE.
+
+Definition IO := itree ioE.
+
+(* ====================================================== *)
+(** *Specification of simple server *)
+(* ====================================================== *)
+From DeepWeb.Lib Require Import Util LinearSpec_Traces LinearSpec_Server.
+From ITree Require Import Traces.
+
+Require Import Coq.ZArith.ZArith.
+From Custom Require Import String.
+
+Definition BUFFER_SIZE : Z := 1024.
+Definition SERVER_PORT : endpoint_id := Endpoint 8000.
+Definition INIT_MSG := repeat_string "0"%char (Z.to_nat BUFFER_SIZE).
+
+Module App.
+Record t : Type := {
+  req_size : nat; (* May be replaced with a parser *)
+  state : Type;
+  initial_state : state;
+  app : state * string -> state * string;
+}.
+End App.
+
+Module Config.
+Record t : Type := {
+  req_size : nat;
+  initial_state : string;
+}.
+End Config.
+
+Import App.
+
+Definition server_app (config: Config.t): App.t :=
+  {|
+    req_size := Config.req_size config;
+    state := string;
+    initial_state := Config.initial_state config;
+    app := fun '(msg) => (msg);
+  |}.
+
+Definition real_app_config : Config.t :=
+  {|
+    Config.req_size := Z.to_nat BUFFER_SIZE;
+    Config.initial_state := INIT_MSG;
+  |}.
+
+Definition real_app := server_app real_app_config.
+
+(* ====================================================== *)
+(** *Specification of simple server *)
+(* ====================================================== *)
+
+From DeepWeb Require Import Spec.Swap_ImplModel.
+
+(* ====================================================== *)
+(* Network events are not compatible with our haskE, because in order to handle
+   these, we have to match the return types (which are not defined in the same
+   way..) *)
+(* Variant networkE : Type -> Type := *)
+(* | Listen : endpoint_id -> networkE unit *)
+(* | Accept : endpoint_id -> networkE connection_id *)
+(* | Shutdown : connection_id -> networkE unit *)
+(* | RecvByte : connection_id -> networkE byte *)
+(* | SendByte : connection_id -> byte -> networkE unit. *)
+
+Section Impl.
+
+  Variable (app : App.t).
+
+  (* Super sketchy subevent handling... This "convert" seems to be too lenient. *)
+  Context `{nondetE -< ioE}.
+  Context `{networkE -< ioE}.
+  Import Monad.MonadNotation.
+
+  Definition send_bytes (c : connection_id) (str : string) : IO.IO unit :=
+    ITree.iter (fun x : string => match x with
+                               | EmptyString => Ret (inr tt)
+                               | String a kx =>
+                                 Vis (convert (SendByte c a)) (fun _ => Ret (inl x))
+                               end
+               ) str.
+
+  (* runConn :: (Socket, SockAddr) -> IO () *)
+  (* runConn (sock, _) = do *)
+  (*   send sock "Hello World!\n" *)
+  (*   close sock *)
+
+  (* runConn specification using networkE and nondetE. networkE is less expressive
+     than haskE (for instance, the "Close" and "Shutdown" are not distinguished.
+  *)
+  Definition runConn (sock : Socket) (addr : NetworkTypes.SockAddr) (sm : SocketMap)
+    : IO.IO (unit * SocketMap) :=
+    or (match connection_of_fd sm sock with (* Successful communication. *)
+        | Some x => ITree.bind (send_bytes x "Hello World")
+                     (fun _ => Vis (convert (Shutdown x)) (fun _ => Ret (tt, sm)))
+        | None => Ret (tt, sm) (* Failed communication. *)
+        end)
+       (Ret (tt, sm)) (* Failed communication. *)
+  .
+
+  (* mainLoop :: Socket -> IO () *)
+  (* mainLoop sock = do *)
+  (*   conn <- accept sock     -- accept a connection and handle it *)
+  (*   runConn conn            -- run our server's logic *)
+  (*   mainLoop sock           -- repeat *)
+  (* Definition mainLoop : NetworkTypes.Socket -> IO.IO unit := *)
+  (* fun (sock : NetworkTypes.Socket) => *)
+  (*   (@ITree.forever IO.ioE unit unit (Network_.accept sock GHC.Base.>>= *)
+  (*     (fun conn => runConn conn))). *)
+
+  (* We can't use DeepWeb to reason about Sockets, because the logic that deals
+     with creating an "observable oracle" and observing only connection events
+     is handled through VST. *)
+  (* Definition mainLoop (sock : Socket) (sm : SocketMap) : IO.IO (unit * SocketMap) := *)
+  (*   match endpoint_of_fd sm sock with *)
+  (*   | Some x => accept_connection x *)
+  (*   | None => Ret tt *)
+  (*   end *)
+  (* . *)
+
+End Impl.
+
+(* ====================================================== *)
+(** *Trace Refinement*)
+(* ====================================================== *)
+
+(* We could get "high-level" traces that are reorderable. *)
+(* DeepWeb's definition of "high-level" is on hiding the abstraction of
+   concurrent and nondeterministic effects. Unfortunately, we still have no way
+   of getting rid of those from our source Haskell program so we can't use these
+   for now.
+ *)
+Definition real_trace := @trace (LinearSpec_Traces.event) byte.
+
+Require Import Coq.Strings.Ascii.
+Local Open Scope char_scope.
+
+Definition network_event_response (e : real_event) (tr : trace) :=
+  match e with
+    | NewConnection id =>
+      (TEventEnd e)
+    | ToServer id b =>
+      (TEventResponse e b tr)
+    | FromServer id b =>
+      (@TEventResponse LinearSpec_Traces.event byte _ e b tr)
+  end.
+
+Inductive network_reordered_ :
+   LinearSpec_NetworkModel.network_state -> real_trace -> real_trace -> Prop :=
+  | ScrambleEmpty : forall ns : LinearSpec_NetworkModel.network_state,
+                    network_reordered_ ns TEnd TEnd
+  | ScrambleServer : forall (ns ns' : LinearSpec_NetworkModel.network_state)
+                       (e : real_event) (tr_server tr_client : trace),
+                     server_transition e ns ns' ->
+                     network_reordered_ ns' tr_server tr_client ->
+                     network_reordered_ ns (network_event_response e tr_server)
+                                        tr_client
+  | ScrambleClient : forall (ns ns' : LinearSpec_NetworkModel.network_state)
+                       (e : real_event) (tr_server tr_client : real_trace),
+                     client_transition e ns ns' ->
+                     network_reordered_ ns' tr_server tr_client ->
+                     network_reordered_ ns tr_server
+                                        (network_event_response e tr_client).
+
+Definition network_reordered := network_reordered_ LinearSpec_NetworkModel.initial_ns.
+
+(* ====================================================== *)
+(** Experiment: Handling into stateT.
+    (Seems inappropriate for modeling nondeterministic and concurrent behavior.) *)
+(* ====================================================== *)
+(** *Network World state
+(* ====================================================== *)
+   We take the conventional perspective of viewing the IO monad
+   as handling effects in the effectful (awkward) _World_, following
+   DeepWeb network model representation.
+   (https://github.com/DeepSpec/DeepWeb/blob/master/src/MiniSwap/Lib/LinearSpec_Interface.v)
+ *)
+
+Section World.
+(* A couple axioms along the way... *)
+
+  (* Assume decidable boolean equality check exists between Sockets. *)
+  Axiom socket_eq : forall (x y : Socket), {x=y}+{x<>y}.
+  Axiom socket_eqb : Socket -> Socket -> bool.
+  Infix "/=?" := socket_eqb (at level 50).
+  (* Assume there is a function that generates new SockAddrs and Sockets.
+    (For `accept`.) *)
+  Axiom newSockAddr : unit -> SockAddr.
+  Axiom newSock : unit -> Socket.
+
+  Definition valid_socket (sl : list Socket) (x : Socket) : bool :=
+    match (List.find (socket_eqb x) sl) with
+    | Some _ => true
+    | _ => false
+    end
+  .
+
+  Notation stateT := ITree.Basics.Basics.Monads.stateT.
+
+  Variable (app : App.t).
+
+  Definition world : Type := SocketMap * list connection * state app.
+
+  Definition handle_send (w : world) (sock : Socket) (b : bytes) :
+    world * Num.Int :=
+    let '(sm, conns, app) := w in
+    match connection_of_fd sm sock with
+    | Some _ => ((sm, conns, app), 1%Z)
+    | None => ((sm, conns, app), 0%Z)
+    end
+  .
+
+  Definition remove_conn (c : connection_id) (cl : list connection) :=
+    cl (* TODO: Filter. *).
+
+  Definition handle_close (w : world) (sock : Socket) : world :=
+    let '(sm, conns, app) := w in
+    match connection_of_fd sm sock with
+    | Some x => (sm, remove_conn x conns, app)
+    | None => w
+    end
+  .
+
+  (* TODO: Implement these handle functions. *)
+  Definition handle_accept (w : world) (sock : Socket) :
+    world * (Socket * SockAddr) :=
+    (w, (sock, newSockAddr tt)).
+
+  Definition handle_listen (w : world) (sock : Socket) (n : Num.Int) : world := w.
+
+  Definition handle_bind (w : world) (sock : Socket) (addr : SockAddr) : world := w.
+
+  Definition handle_socket (w : world) : world * Socket :=
+    (w, newSock tt).
+
+  Definition handle_setSocketOption (w : world) : world := w. 
+
+  (* To model the world state, we wish to interpret these events into a
+    stateT monad with world information. *)
+  Definition h_network {E} : haskE ~> stateT world (itree E) :=
+    fun _ e w =>
+      match e with
+      | SendE s b => Ret (handle_send w s b)
+      | CloseE s => Ret (handle_close w s, tt)
+      | AcceptE s => Ret (handle_accept w s)
+      | ListenE s n => Ret (handle_listen w s n, tt)
+      | BindE s a => Ret (handle_bind w s a, tt)
+      | SocketE _ _ _ => Ret (handle_socket w)
+      | SetSocketOptionE f s n => Ret (handle_setSocketOption w, tt)
+      end.
+
+  (* Old version... *)
+  (*       if valid_socket skt s then *)
+  (*         Ret ((sm, clnt, skt, (s, x)::msgs), 1% Z) *)
+  (*       else *)
+  (*         Ret ((srv, clnt, skt, msgs), 0%Z) *)
+  (*     | CloseE s => *)
+  (*       if valid_socket skt s then *)
+  (*         Ret ((srv, clnt, remove socket_eq s skt, msgs), tt) *)
+  (*       else *)
+  (*         Ret ((srv, clnt, skt, msgs), tt) *)
+  (*     | AcceptE s => *)
+  (*       if valid_socket skt s then *)
+  (*         match srv with *)
+  (*         | (ls, n, true) => *)
+  (*           if length ls <? n then *)
+  (*             Ret (((s::ls, n, true), clnt, skt, msgs), (s, newSockAddr tt)) *)
+  (*           else *)
+  (*             Ret (((s::(removelast ls), n, true), clnt, skt, msgs), *)
+  (*                 (s, newSockAddr tt)) *)
+  (*         | (_, _, _) => (Ret ((srv, clnt, skt, msgs), (s, newSockAddr tt))) *)
+  (*         end *)
+  (*       else *)
+  (*         Ret ((srv, clnt, skt, msgs), (s, newSockAddr tt)) *)
+  (*     | ListenE s n => (* ListenE mutates "global" connection max count... *) *)
+  (*       if valid_socket skt s then *)
+  (*         match srv with *)
+  (*         | (ls, _, false) => Ret (((ls, Z.to_nat n, true), clnt, skt, msgs), tt) *)
+  (*         | (_, _, _) => Ret ((srv, clnt, skt, msgs), tt) *)
+  (*         end *)
+  (*       else *)
+  (*         Ret ((srv, clnt, skt, msgs), tt) *)
+  (*     | BindE s a => *)
+  (*       if valid_socket skt s then *)
+  (*         match srv with *)
+  (*         | (ls, _, true) => Ret ((srv, clnt, skt, msgs), tt) *)
+  (*         | (_, _, _) => Ret ((srv, clnt, skt, msgs), tt) *)
+  (*         end *)
+  (*       else *)
+  (*         Ret ((srv, clnt, skt, msgs), tt) *)
+  (*     (* Takes in dummy socket generator... *) *)
+  (*     | SocketE _ _ _ => Ret ((srv, clnt, (newSock tt)::skt, msgs), newSock tt) *)
+  (*     (* Ignore this Socket representation, for now. *) *)
+  (*     | SetSocketOptionE f s n => Ret ((srv, clnt, skt, msgs), tt) *)
+  (*     end *)
+  (* . *)
+
+  (* Since there is only one event type (network), handling IO is equivalent to
+    handling networks. *)
+  Definition h_io {E} : ioE ~> stateT world (itree E) := h_network.
+
+  Definition interp_io {E A} (t : itree ioE A) : stateT world (itree E) A :=
+    interp h_io t.
+
+End World.
+
+(* ====================================================== *)
+(* Functor/Applicative/Monad laws, taken from wc example. *)
+
+Section Functors.
+
+  Variable f : Type -> Type.
+
+  Context `{Functor.Functor f}.
+
+  Global Instance Functor_Functor : Functor f :=
+    fun _ X =>
+      X {| fmap__ := fun a b : Type => Functor.fmap;
+           op_zlzd____ := fun a b : Type => Functor.fmap ∘ const
+        |}.
+
+  Section Applicatives.
+
+    Context `{Applicative.Applicative f}.
+
+    Global Instance Applicative_Applicative : Applicative f :=
+      fun _ X =>
+        X {| liftA2__ := fun a b c f x y => Applicative.ap (fmap f x) y;
+             op_zlztzg____ := fun a b => Applicative.ap ;
+             op_ztzg____ := fun a b x y => Applicative.ap (id <$ x) y;
+             pure__ := fun a => Applicative.pure
+          |}.
+
+    Section Monads.
+
+      Context `{Monad.Monad f}.
+
+      Global Instance Monad_Monad : Monad f :=
+        fun _ X =>
+          X {| op_zgzg____ := fun a b x y => Monad.bind x (fun _ => y);
+               op_zgzgze____ := fun a b => Monad.bind ;
+               return___ := fun a => Monad.ret
+            |}.
+
+    End Monads.
+  End Applicatives.
+End Functors.
+
+Instance Functor_IO : Functor IO := Functor_Functor IO.
+Instance Applicative_IO : Applicative IO := Applicative_Applicative IO.
+Instance Monad_IO : Monad IO := Monad_Monad IO.
