examples/http/manual/ImplModel.v
@@ -1,0 +1,73 @@
+Require Import ServerDefs.
+From Coq Require Import String.
+From ExtLib Require Import Monad.
+Import MonadNotation.
+Open Scope monad_scope.
+
+Section Impl.
+
+(** *Sockets, Endpoints and Connection IDs
+
+    A *socket* is one endpoint of a two-way communication
+    link between two programs running on the network. A socket
+    is bound to a port number so that the TCP layer can
+    identify the application that data is destined to be sent to.
+
+    From the standpoint of the network state (the oracle that
+    we wish to specify), we do not care for the representation
+    of sockets. Rather, we care about the state of the connection
+    endpoints themselves.
+
+    For BOUND and LISTENING sockets, we give `endpoint_ID`s,
+    which correspond to sockets on the server side.
+
+    CONNECTED sockets have `connection_id`s, which is assigned
+    to clients.
+
+    CLOSED and OPENED sockets have no reperesntation in our
+    network state oracle.
+ *)
+
+  Inductive connection_state : Type :=
+    RECVING | SENDING | DONE | DELETED.
+
+  Record connection : Type :=
+    {
+      conn_id : connection_id;
+      conn_request : string;
+      conn_response : string;
+      conn_response_bytes_sent : nat;
+      conn_state : connection_state
+    }.
+
+(* runConn :: (Socket, SockAddr) -> IO () *)
+(* runConn (sock, _) = do *)
+(*   -- Send data to socket. Socket must be connected to a remote socket. returns *)
+(*   -- number of bytes sent. Apps are responsible for ensuring all data has been sent. *)
+(*   send sock "Hello World!\n" *)
+(*   -- `close` does not throw exceptions *)
+(*   close sock *)
+
+  (* Definition runConn *)
+  (*   : (NetworkTypes.Socket * NetworkTypes.SockAddr)%type -> IO.IO unit := *)
+  (*   fun '(pair sock _) => *)
+  (*     Network_.send sock (GHC.Base.hs_string__ "Hello World!") GHC.Base.>> *)
+  (*     Network_.close sock. *)
+
+  (* Definition runConn (addr : endpoint_id): *)
+  (*   itree socketE (option connection) := *)
+  (*   or (client_conn <- send connection_id "Hello World!\n"). *)
+
+
+Definition mainLoop : NetworkTypes.Socket -> IO.IO unit :=
+  fun (sock : NetworkTypes.Socket) =>
+    (@ITree.forever IO.ioE unit unit (Network_.accept sock GHC.Base.>>=
+      (fun conn => runConn conn))).
+
+Definition main : IO.IO unit :=
+  Network_.socket NetworkTypes.AF_INET NetworkTypes.Stream #0 GHC.Base.>>=
+  (fun sock =>
+     Network_.setSocketOption sock NetworkTypes.ReuseAddr #1 GHC.Base.>>
+     (Network_.bind sock (NetworkTypes.SockAddrInet #4242 NetworkTypes.iNADDR_ANY)
+      GHC.Base.>>
+      (Network_.listen sock #2 GHC.Base.>> mainLoop sock))).
