examples/http/manual/LinearSpec.v
@@ -1,0 +1,58 @@
+(** * Linear specification of hello server *)
+
+(* The effect type [specE] used by the specification is defined
+   in [SpecEffect] as
+
+       Definition specE := failureE +' nondetE +' observerE.
+
+   where [observerE] is defined there, [failureE] and [nondetE]
+   are general-purpose exception and nondeterminism effects from
+   the InteractionTree library.
+ *)
+
+From ITree Require Import
+     ITree
+     Events.Nondeterminism.
+
+From Coq Require Import
+     Ascii String List PArith ZArith.
+From Coq Require Fin.
+
+From QuickChick Require Import QuickChick.
+From ExtLib Require Import Monad.
+Open Scope monad_scope.
+Require Import ServerDefs StringLib SpecEffect.
+Import ListNotations MonadNotation.
+
+(* begin hide *)
+Set Warnings "-extraction-opaque-accessed,-extraction".
+(* end hide *)
+
+Section LinearSpec.
+Variable (app : App.t).
+
+(* ====================================================== *)
+(** *Linear Specification *)
+(* ====================================================== *)
+CoFixpoint linear_spec'
+           (conns : list connection_id)
+           (s : App.state app)
+  : itree specE unit :=
+    or ( (* Accept a new connection. *)
+      c <- obs_connect;;
+      linear_spec' (c :: conns) s
+    )
+    ( (* Send Hello World message from server. *)
+      c <- choose conns;;
+      let '(s', resp) := App.app app s in
+      obs_msg_from_server c resp;;
+      linear_spec' conns s'
+    ).
+
+(* Top-level spec. *)
+Definition linear_spec :=
+  linear_spec' [] (App.initial_state app).
+
+End LinearSpec.
+
+Definition hello_app_spec := linear_spec hello_app.
