examples/http/manual/Network_.v
@@ -2,25 +2,44 @@
 From ITree Require Import ITree.
 Require Import NetworkTypes.
 Require Import IO.
+Require Import StringLib.
+From Coq Require Import Strings.String.
+Require Import GHC.Char.
 
-Definition send : Socket -> Base.String -> IO Num.Int :=
-  fun s x => embed (SendE s x).
+Require Import NArith.
 
-Definition close : Socket -> IO unit :=
-  fun s => embed (CloseE s).
+Fixpoint string_hs__ (s : Base.String) : string :=
+  match s with
+  | nil => EmptyString
+  | cons c s  => String (ascii_of_nat (N.to_nat c)) (string_hs__ s)
+  end.
 
-Definition accept : Socket -> IO (Socket * SockAddr) :=
-  fun s => embed (AcceptE s).
+Coercion Base.hs_string__ : string >-> Base.String.
+Coercion string_hs__ : Base.String >-> string.
 
-Definition listen : Socket -> Num.Int -> IO unit :=
-  fun s x => embed (ListenE s x).
+Section NetworkEmbed.
 
-Definition bind : Socket -> SockAddr -> IO unit :=
-  fun s x => embed (BindE s x).
 
-Definition setSocketOption :
-  Socket -> SocketOption -> Num.Int -> IO unit :=
-  fun s x y => embed (SetSocketOptionE s x y).
+  Definition send : Socket -> Base.String -> IO Num.Int :=
+    fun s x => embed (SendE s x).
 
-Definition socket : Family -> SocketType -> Num.Int -> IO Socket :=
-  fun f s x => embed (SocketE f s x).
+  Definition close : Socket -> IO unit :=
+    fun s => embed (CloseE s).
+
+  Definition accept : Socket -> IO (Socket * SockAddr) :=
+    fun s => embed (AcceptE s).
+
+  Definition listen : Socket -> Num.Int -> IO unit :=
+    fun s x => embed (ListenE s x).
+
+  Definition bind : Socket -> SockAddr -> IO unit :=
+    fun s x => embed (BindE s x).
+
+  Definition setSocketOption :
+    Socket -> SocketOption -> Num.Int -> IO unit :=
+    fun s x y => embed (SetSocketOptionE s x y).
+
+  Definition socket : Family -> SocketType -> Num.Int -> IO Socket :=
+    fun f s x => embed (SocketE f s x).
+
+End NetworkEmbed.
