examples/http/manual/ServerDefs.v
@@ -1,0 +1,91 @@
+(* ====================================================== *)
+(** *Specification of simple server *)
+(* ====================================================== *)
+From ITree Require Import Traces.
+
+Require Import Coq.ZArith.ZArith.
+Require Import StringLib.
+
+(* ====================================================== *)
+(** *Modeling Network App State
+
+    The network state contains information about the
+    buffer size, initial state, and the state transitions
+    that define the behavior of the application.
+ *)
+(* ====================================================== *)
+
+(** *Sockets, Endpoints and Connection IDs
+
+    A *socket* is one endpoint of a two-way communication
+    link between two programs running on the network. A socket
+    is bound to a port number so that the TCP layer can
+    identify the application that data is destined to be sent to.
+
+    From the standpoint of the network state (the oracle that
+    we wish to specify), we do not care for the representation
+    of sockets. Rather, we care about the state of the connection
+    endpoints themselves.
+
+    For BOUND and LISTENING sockets, we give `endpoint_ID`s,
+    which correspond to sockets on the server side.
+
+    CONNECTED sockets have `connection_id`s, which is assigned
+    to clients.  
+
+    CLOSED and OPENED sockets have no reperesntation in our
+    network state oracle.
+ *)
+
+Inductive connection_id : Type := Connection (c : nat).
+Record endpoint_id : Type := Endpoint { port_number : Z; }.
+
+(* Assume buffer size to be 1024 bytes. *)
+Definition BUFFER_SIZE : Z := 1024.
+Definition SERVER_PORT : endpoint_id := Endpoint 4242.
+
+Definition byte := Ascii.ascii.
+Definition bytes := string.
+Definition hello_message : bytes := "Hello, World!".
+
+Definition
+  INIT_MSG := hello_message ++ repeat_string "0"%char (Z.to_nat BUFFER_SIZE -
+                                                       (length hello_message)).
+
+Module App.
+Record t : Type := {
+  req_size : nat;
+  state : Type;
+  initial_state : state;
+  app : state -> state * bytes;
+}.
+End App.
+
+Module Config.
+Record t : Type := {
+  req_size : nat;
+  initial_state : string;
+}.
+End Config.
+
+Section HelloApp.
+Import App.
+
+(* Constant state: server always sends Hello World message *)
+Definition network_app (config: Config.t): App.t :=
+  {|
+    req_size := Config.req_size config;
+    state := string;
+    initial_state := Config.initial_state config;
+    app := fun 'state => (state, state);
+  |}.
+
+Definition hello_app_config : Config.t :=
+  {|
+    Config.req_size := Z.to_nat BUFFER_SIZE;
+    Config.initial_state := INIT_MSG;
+  |}.
+
+Definition hello_app := network_app hello_app_config.
+
+End HelloApp.
