examples/http/manual/SpecEffect.v
@@ -1,0 +1,113 @@
+From ITree Require Import
+     ITree
+     Events.Nondeterminism
+     Events.Exception
+     Subevent.
+
+From Coq Require Import
+     Ascii String List PArith ZArith.
+From Coq Require Fin.
+
+From QuickChick Require Import QuickChick.
+Open Scope monad_scope.
+Require Import ServerDefs StringLib.
+From ExtLib Require Import Monad.
+Import ListNotations MonadNotation.
+
+Section SpecEffects.
+
+  Generalizable Variable E.
+
+(* ====================================================== *)
+(** *Specification Effects *)
+(* ====================================================== *)
+
+(** The type of observations that can be made by the spec. *)
+Inductive observerE : Type -> Type :=
+| (* Observe the creation of a new connection *)
+  ObsConnect : observerE connection_id
+
+| (* Observe a byte going into the server on a particular
+     connection *)
+  ObsToServer : connection_id -> observerE byte
+
+  (* Observe a byte going out of the server.  This action can return
+     [None], indicating a "hole" as a way to hypothesize that the
+     server sent some message we haven't yet received, so we can keep
+     testing the rest of the trace. *)
+| ObsFromServer : connection_id -> observerE (option byte).
+
+(* The [ObsFromServer] effect returns an [option].
+   [None] is a "hole" in the observed trace, it represents a
+   message hypothetically sent by the server and that we haven't
+   yet received. These holes allow us to keep exploring an
+   observer even in the presence of partial outputs from the
+   server. *)
+
+(* Note: The spec writer must be careful that, if a trace with
+   holes is rejected, then it must also be for any substitution
+   of actual values for those holes. *)
+
+Definition failureE := exceptE string.
+
+Definition fail `{failureE -< E} {R} (reason : string) : itree E R
+  := vis (Throw reason) (fun v : void => match v with end).
+
+(* This can fail if the list is empty. *)
+Definition choose {E} `{failureE -< E} `{nondetE -< E} {X}
+  : list X -> itree E X := fix choose' xs : itree E X :=
+  match xs with
+  | [] => fail "choose: No choice left"
+  | x :: xs =>
+    or (Ret x) (choose' xs)
+  end.
+
+(* Definition fail (err : string) := trigger (Throw err) *)
+Definition specE := nondetE +' observerE +' failureE.
+
+Definition obs_connect {E} `{observerE -< E} : itree E connection_id :=
+  embed ObsConnect.
+
+Definition obs_to_server {E} `{observerE -< E} :
+  connection_id -> itree E byte :=
+  embed ObsToServer.
+
+Definition obs_from_server {E} `{observerE -< E} :
+  connection_id -> itree E (option byte) :=
+  embed ObsFromServer.
+
+(* Make an assertion on a value, if it exists. *)
+Definition assert_on {E A} `{failureE -< E} `{nondetE -< E}
+           (r : string) (oa : option A) (check : A -> bool) :
+  itree E unit :=
+  match oa with
+  | None => ret tt
+  | Some a =>
+    if check a then ret tt else fail ("assertion failed: " ++ r)
+  end.
+
+(* Observe a message of length [n] sent to the server. *)
+Fixpoint obs_msg_to_server `{observerE -< E}
+         (n : nat) (c : connection_id) : itree E bytes :=
+  match n with
+  | O => ret ""
+  | S n =>
+    b <- obs_to_server c;;
+    bs <- obs_msg_to_server n c;;
+    ret (b ::: bs)
+  end%string.
+
+(* Observe a message of length [n] received from the server. *)
+Fixpoint obs_msg_from_server
+         `{observerE -< E} `{failureE -< E} `{nondetE -< E}
+         (c : connection_id) (msg : bytes) :
+  itree E unit :=
+  match msg with
+  | "" => ret tt
+  | b0 ::: msg =>
+    ob <- obs_from_server c;;
+    (assert_on "bytes must match" ob (fun b1 => (b1 = b0 ?)));;
+    obs_msg_from_server c msg
+  end%string.
+
+End SpecEffects.
