examples/http/lib/StringLib.v
@@ -1,0 +1,1 @@
+../manual/StringLib.v
